Refactor, using lists now

src/PTLC.lean
@@ -1,12 +1,36 @@
--- Definition of the lambda cube --
+import Init.Data.Nat.Basic
 
--- Nat --
-inductive nat : Type
-  | zero : nat
-  | succ : nat → nat
+--Presorts--
+-- Those are lists of natural numbers
+inductive pre_sort : Type
+  | nil : pre_sort
+  | append : (n : nat) → (l: pre_sort) → pre_sort
 
---Sorts--
-inductive sort : Type
-  | nil : sort
-  | append : sort → sort → sort
-  | ▵ : Type
+-- Lists --
+inductive list (T : Type): Type
+  | nil : list T
+  | append : (t : T) → (l : list T) → list T
+
+notation "[]" => list.nil
+notation t","l => list.append t l
+
+inductive not_in (t : T) : list T → Prop
+  | nil : not_in t []
+  | next : (t ≠ t₀) → not_in t l → not_in t (t₀ , l)
+
+inductive no_duplicates (T : Type) : list T → Prop
+  | nil : no_duplicates T nil
+  | head (t : T) (l : list T): not_in t l → no_duplicates T (t , l)
+
+-- Some test for lists of integers --
+---------------------------------------------------------
+def list₀ : list Nat := (0 , (1 , []))
+
+-- Proof that there is no duplicates in list₀ --
+example : no_duplicates Nat list₀ := by
+  unfold list₀
+  apply no_duplicates.head
+  apply not_in.next
+  simp
+  apply not_in.nil
+--------------------------------------------------------
